theories/tree_td.v
@@ -17,11 +17,46 @@ Instance is_tree_leaf_hint t :
 HINT ε₁ ✱ [- ; ⌜t = Leaf⌝] ⊫ [id]; is_tree t NULL ✱ [⌜t = Leaf⌝].
 Proof. iSteps. Qed.
 
+(* Diaframe deconstructs arrays like p ↦∗ [ l'; #x; r'] into parts,
+   so we can only check that the components are correct. *)
 #[export]
 Instance is_tree_node_hint (p : loc) (x : Z) (l_r l_l : val) t :
-HINT p ↦∗ [ l_l; #x; l_r] ✱ [ l r ; is_tree l l_l ∗ is_tree r l_r ∗ ⌜t = Node l x r⌝]
+HINT ε₁ ✱ [ l r ; (p +ₗ 0) ↦ l_l ∗ (p +ₗ 1) ↦ #x ∗ (p +ₗ 2) ↦ l_r ∗ is_tree l l_l ∗ is_tree r l_r ∗ ⌜t = Node l x r⌝]
   ⊫ [id]; is_tree t #p ✱ [⌜t = Node l x r⌝].
-Proof. iSteps. Qed.
+Proof. unfold is_tree, array. simpl. iSteps. Qed.
+
+(* We want to figure out if a tree is a Leaf or a Node from the "t != NULL" check.
+   To achieve this, Ike Mulder wrote this typeclass inference code. *)
+Definition is_tree_value_at (t' : tree) (treev : val) : Prop :=
+  match t' with
+  | Leaf => treev = NULL
+  | Node l x r => ∃ (p : loc),
+      treev = #p
+  end.
+
+#[export]
+Instance is_tred_none t : MergablePersist (is_tree t NULL) (fun p Pin Pout =>
+  TCAnd (TCEq Pin (empty_hyp_first))
+        (TCEq Pout (bi_pure (t= Leaf)))) | 5.
+Proof. unfold MergablePersist.
+  move => p Pin Pout [-> ->].
+  destruct t; iSteps. Qed. 
+
+#[export]
+Instance is_tred_always t tv : MergablePersist (is_tree t tv) (fun p Pin Pout =>
+    TCAnd (TCEq Pin (empty_hyp_first))
+          (TCEq Pout (bi_pure (is_tree_value_at t tv)))) | 50.
+Proof. unfold MergablePersist. move => p Pin Pout [-> ->].
+  destruct t; iSteps. Qed.
+
+Lemma simplifytreenotnil t tv : 
+  is_tree_value_at t tv ->
+  SimplifyPureHyp (tv ≠ NULL) (exists (l : loc), tv = #l /\ exists l x r, t = Node l x r).
+Proof. unfold SolveSepSideCondition, SimplifyPureHyp. destruct t; naive_solver. Qed.
+
+#[export]
+Hint Extern 4 (SimplifyPureHyp (_ ≠ NULL) _) => 
+  eapply simplifytreenotnil; eauto : typeclass_instances.
 
 Definition is_root_tree (t : root_tree) (v : val) : iProp Σ :=
   match t with
@@ -30,9 +65,9 @@ Definition is_root_tree (t : root_tree) (v : val) : iProp Σ :=
 
 #[export]
 Instance is_root_tree_root_hint (p : loc) (x : Z) (l_r l_l : val) t :
-HINT p ↦∗ [ l_l; #x; l_r] ✱ [ l r ; is_tree l l_l ∗ is_tree r l_r ∗ ⌜t = Root l x r⌝]
+HINT ε₁ ✱ [ l r ; (p +ₗ 0) ↦ l_l ∗ (p +ₗ 1) ↦ #x ∗ (p +ₗ 2) ↦ l_r ∗ is_tree l l_l ∗ is_tree r l_r ∗ ⌜t = Root l x r⌝]
   ⊫ [id]; is_root_tree t #p ✱ [⌜t = Root l x r⌝].
-Proof. iSteps. Qed.
+Proof. unfold is_root_tree, array. simpl. iSteps. Qed.
 
 Definition harray (l : loc) (k : nat) (dq : dfrac) (vs : list val) : iProp Σ :=
   [∗ list] i ↦ v ∈ vs, ⌜i = k⌝ ∨ (l +ₗ i) ↦{dq} v.
@@ -58,15 +93,15 @@ Definition is_ctx0 (z : ctx) (p' : loc) (h : loc) : iProp Σ :=
 
 #[export]
 Instance is_ctx0_node0_hint (p : loc) (x : Z) (r' : val) (z : ctx) :
-HINT (p +ₗ 1%nat) ↦∗ [ #x; r' ] ✱ [ r ; is_tree r r' ∗ ⌜z = Node0 Hole x r⌝]
+HINT ε₁ ✱ [ r ; (p +ₗ 1%nat) ↦ #x ∗ (p +ₗ 2%nat) ↦ r' ∗ is_tree r r' ∗ ⌜z = Node0 Hole x r⌝]
   ⊫ [id]; is_ctx0 z p (p +ₗ 0%nat) ✱ [⌜z = Node0 Hole x r⌝].
 Proof. iSteps. cbn. iSteps. Qed.
 
 #[export]
 Instance is_ctx0_node2_hint (p : loc) (x : Z) (l' : val) (z : ctx) :
-HINT p ↦∗ [ l'; #x ] ✱ [ l ; is_tree l l' ∗ ⌜z = Node2 l x Hole⌝]
+HINT ε₁ ✱ [ l ; (p +ₗ 0%nat) ↦ l' ∗ (p +ₗ 1%nat) ↦ #x ∗ is_tree l l' ∗ ⌜z = Node2 l x Hole⌝]
   ⊫ [id]; is_ctx0 z p (p +ₗ 2%nat) ✱ [⌜z = Node2 l x Hole⌝].
-Proof. iSteps. cbn. iSteps. Qed.
+Proof. iSteps. unfold array, harray. iSteps. Qed.
 
 #[export]
 Instance is_ctx_hole_hint z p :
@@ -76,24 +111,19 @@ Proof. iSteps. Qed.
 Lemma ctx_of_ctx0 (z : ctx) (p : loc) (h : loc) :
     (∃ (p' : loc), p ↦ #p' ∗ is_ctx0 z p' h) -∗ is_ctx z p h.
 Proof.
-  iIntros "[%p' [Hp Hz]]". iInduction z as [|z x r|l x z] "IH" forall (p h).
-  - iDecompose "Hz".
-  - iDecompose "Hz". iExists p', x. iSteps.
-  - iDecompose "Hz". iExists p', x0. iSteps.
+  iIntros "[%p' [? Hz]]". iInduction z as [] "" forall (p h); iDecompose "Hz"; iSteps.
 Qed.
 
 Lemma tree_of_ctx (z : ctx) (t : tree) (zv : loc) (hv : loc) (tv : val) :
     is_ctx z zv hv ∗ hv ↦ tv ∗ is_tree t tv -∗ ∃ zv', zv ↦ zv' ∗ is_tree (plug z t) zv'.
 Proof.
   iIntros "[Hz [Hhv Ht]]". iInduction z as [|z x r|l x z] "IH" forall (zv hv t).
-  - iDecompose "Hz". iExists tv. iFrame.
-  - iDecompose "Hz". iExists #x. iFrame.
-    iAssert (∃ l', (Loc.add x 0%nat) ↦ l' ∗ is_tree (plug z t) l')%I with "[H5 Ht Hhv]" as "[%l' [Hl' Hl]]".
-      { iSteps. }
+  - iDecompose "Hz". iSteps.
+  - iDecompose "Hz" as (? ? ?) "H1 H2 H3 H4". iExists #x. iFrame.
+    iPoseProof ("IH" $! (Loc.add x 0) hv t with "H3 Hhv Ht") as "[%l' [H1' H2']]".
     iExists x, l', x0. unfold array, harray. iSteps.
-  - iDecompose "Hz". iExists #x0. iFrame.
-    iAssert (∃ r', (Loc.add x0 2%nat) ↦ r' ∗ is_tree (plug z t) r')%I with "[H5 Ht Hhv]" as "[%r' [Hr' Hr]]".
-      { iSteps. }
+  - iDecompose "Hz" as (? ? ?) "H1 H2 H3 H4". iExists #x0. iFrame.
+    iPoseProof ("IH" $! (Loc.add x0 2) hv t with "H3 Hhv Ht") as "[%r' [H1' H2']]".
     iExists x0, x1, r'. unfold array, harray. iSteps.
 Qed.
 
@@ -103,9 +133,9 @@ Proof.
   iIntros "[Hz [Hhv Ht]]". iInduction z1 as [|z x r|l x z] "IH" forall (zv1 hv1 z2 zv2 hv2).
   - iDecompose "Hz". iExists zv2. iFrame.
   - iDecompose "Hz". iExists x. iFrame. iExists x0. iFrame.
-    iApply (ctx_of_ctx0). iSteps.
+    iApply (ctx_of_ctx0). iSteps. repeat rewrite (Loc.add_0). iSteps.
   - iDecompose "Hz". iExists x0. iFrame. iExists x1. iFrame.
-    iApply (ctx_of_ctx0). iSteps.
+    iApply (ctx_of_ctx0). iSteps. repeat rewrite (Loc.add_0). iSteps.
 Qed.
 
 Lemma ctx_of_ctx (z1 : ctx) (z2 : ctx) (zv1 : loc) (hv1 : loc) (zv2 : loc) (hv2 : loc) :
@@ -127,7 +157,15 @@ Instance tree_of_ctx_hint z t t' zv hv tv :
 HINT is_ctx z zv hv ✱ [- ; hv ↦ tv ∗ is_tree t tv ∗ ⌜t' = plug z t⌝]
   ⊫ [id] zv'; zv ↦ zv' ✱ [ is_tree t' zv' ∗ ⌜t' = plug z t⌝].
 Proof.
-  iStartProof. simpl. iStep. iPoseProof (tree_of_ctx) as "?". iSteps.
+  iSteps. iPoseProof (tree_of_ctx z t zv hv) as "?". iSteps.
+Qed.
+
+#[export]
+Instance tree_of_ctx_df_hint z t t' zv hv tv :
+HINT is_ctx z zv hv ✱ [- ; hv ↦ tv ∗ is_tree t tv ∗ ⌜t' = plug z t⌝]
+  ⊫ [id] zv' df; zv ↦{ df } zv' ✱ [ is_tree t' zv' ∗ ⌜t' = plug z t⌝].
+Proof.
+  iSteps. iPoseProof (tree_of_ctx z t zv hv) as "?". iSteps.
 Qed.
 
 Notation "e1 '->left'" :=
