theories/reverse.v
@@ -38,12 +38,14 @@ Proof. iSteps. Qed.
 
 #[export]
 Instance is_list_cons_hint (p : loc) (x : Z) (l_acc : val) t :
-HINT p ↦∗ [ #x; l_acc] ✱ [ acc ; is_list acc l_acc ∗ ⌜t = x :: acc⌝]
+HINT ε₁ ✱ [ acc ; (p +ₗ 0) ↦ #x ∗ (p +ₗ 1) ↦ l_acc ∗ is_list acc l_acc ∗ ⌜t = x :: acc⌝]
   ⊫ [id]; is_list t #p ✱ [⌜t = x :: acc⌝].
-Proof. iSteps. Qed.
+Proof. unfold is_list, array. iSteps. Qed.
 
 Lemma heap_reverse_correct (xsv : val) (xs : list Z) :
-    {{{ is_list xs xsv }}} heap_reverse (ref xsv) {{{ v, RET v; is_list (reverse xs []) v }}}.
+    {{{ is_list xs xsv }}}
+    heap_reverse (ref xsv)
+    {{{ v, RET v; is_list (reverse xs []) v }}}.
 Proof.
   wp_begin "Hxs"; curr. wp_var prev.          (* Set up the program with variables curr and prev *)
   wp_while (∃ xs' acc' prevv currv,           (* This is the main loop invariant: *)
@@ -51,12 +53,7 @@ Proof.
     ∗ prev ↦ prevv ∗ is_list acc' prevv       (* - prev points to an Iris list corresponding to acc' *)
     ∗ ⌜reverse xs [] = reverse xs' acc'⌝)%I.  (* - and xs', acc' correspond to one iteration of the functional program *)
   - iModIntro. iIntros "[%xs' [% [% [% [? [Hxs [? [? ->]]]]]]]]".
-    destruct xs'; iDecompose "Hxs".           (* Split the current list as in the `match` statement *)
-     { wp_type. }                             (* If the list is empty, the loop finishes and we are done *)
-     { wp_heap.                               (* Otherwise, we evaluate `curr != NULL` *)
-       wp_enter_loop.                         (* curr is not null and we enter the loop *)
-       wp_heap.                               (* We complete the assignments of the main loop body *)
-       wp_type. }                             (* We show that the loop invariant is maintained *)
+    destruct xs'; iDecompose "Hxs"; wp_type.  (* Split the current list as in the `match` statement. *)
   - wp_type.                                  (* We show that the loop invarint is true at the start. *)
 Qed.
 
