theories/splay_td.v
@@ -118,8 +118,7 @@ Lemma heap_td_insert_correct (i : Z) (tv : val) (t : tree) :
     {{{ v, RET v; is_tree (td_insert i t) v }}}.
 Proof.
   wp_begin "Ht"; ref_i, tree.
-  wp_alloc lctx as "Hlctx". wp_let.
-  wp_alloc rctx as "Hrctx". wp_let.
+  wp_alloc lctx as "Hlctx". wp_let. wp_alloc rctx as "Hrctx". wp_let.
   wp_var lhole. wp_var rhole. wp_while_true "H"
     (∃ lz' l (x : Z) rz' r treev (lhv rhv : loc) lhvv rhvv,
             tree ↦ treev ∗ is_tree (Node l x r) treev ∗ ref_i ↦ #i
@@ -131,31 +130,21 @@ Proof.
             ∗ lhole ↦ #lhv ∗ lhv ↦ lhvv ∗ is_ctx lz' lctx lhv
             ∗ rhole ↦ #rhv ∗ rhv ↦ rhvv ∗ is_ctx rz' rctx rhv
             ∗ ⌜td_insert_go i Hole Hole t = td_insert_go i lz' rz' t'⌝)%I.
-  - unfold td_insert.
-    iDestruct "H" as (lz' l x rz' r ? ? ? ? ?)
-      "[? [Ht [? [? [Hlhv [Hlz [? [Hrhv [Hrz ->]]]]]]]]]".
-    iDestruct "Ht" as (? ? ?) "[-> [? [Hl Hr]]]". unfold assemble. wp_heap.
-    iAssert (∃ tl, lctx ↦ tl ∗ is_tree (plug lz' l) tl)%I
-      with "[Hlz Hlhv Hl]" as "[%tl [Hlz Hl]]". { wp_type. }
-    iAssert (∃ tr, rctx ↦ tr ∗ is_tree (plug rz' r) tr)%I
-      with "[Hrz Hrhv Hr]" as "[%tr [Hrv Hr]]". { wp_type. }
-    wp_heap. wp_type.
-  - iDestruct "H" as (? ? t' ? ? ? ? ?) "[? [Ht [? [? [? [? [? [? [? ->]]]]]]]]]".
+  - unfold td_insert. iDecompose "H". unfold assemble.
+    wp_type. now rewrite H2.
+  - iDestruct "H" as (? ? t' ? ? ? ? ?) "(? & Ht & ? & ? & ? & ? & ? & ? & ? & ->)".
     unfold rotate_right, rotate_left, link_right, link_left.
     destruct t' as [|l x r].
     + iDecompose "Ht". wp_heap. wp_type.
-    + iDestruct "Ht" as (? ? ?) "[-> [? [Hl Hr]]]". wp_heap.
-      unfold td_insert_go at 1. case_bool_decide; wp_heap. 
-      { wp_type. }
+    + iDestruct "Ht" as (? ? ?) "(-> & ? & Hl & Hr)". wp_heap.
+      unfold td_insert_go at 1. case_bool_decide; wp_heap. { wp_type. }
       { case_bool_decide; wp_heap.
         - destruct l; iDecompose "Hl".
           + wp_heap. wp_type.
-          + wp_heap. case_bool_decide; wp_heap.
-            { wp_type. } { case_bool_decide; wp_heap; wp_type. }
+          + wp_heap. case_bool_decide; wp_heap; wp_type.
         - destruct r; iDecompose "Hr".
           + wp_heap. wp_type.
-          + wp_heap. case_bool_decide; wp_heap.
-            { wp_type. } { case_bool_decide; wp_heap; wp_type; iExFalso; lia. } }
+          + wp_heap. case_bool_decide; wp_heap; wp_type; iExFalso; lia. }
   - wp_type.
 Qed.
 
