theories/tree_bu.v
@@ -16,11 +16,13 @@ Instance is_tree_leaf_hint t :
 HINT ε₁ ✱ [- ; ⌜t = Leaf⌝] ⊫ [id]; is_tree t NULL ✱ [⌜t = Leaf⌝].
 Proof. iSteps. Qed.
 
+(* Diaframe deconstructs arrays like p ↦∗ [ l'; #x; r'] into parts,
+   so we can only check that the components are correct. *)
 #[export]
 Instance is_tree_node_hint (p : loc) (x : Z) (l_r l_l : val) t :
-HINT p ↦∗ [ #1; l_l; #x; l_r] ✱ [ l r ; is_tree l l_l ∗ is_tree r l_r ∗ ⌜t = Node l x r⌝]
+HINT ε₁ ✱ [ l r; (p +ₗ 0) ↦ #1 ∗ (p +ₗ 1) ↦ l_l ∗ (p +ₗ 2) ↦ #x ∗ (p +ₗ 3) ↦ l_r ∗ is_tree l l_l ∗ is_tree r l_r ∗ ⌜t = Node l x r⌝]
   ⊫ [id]; is_tree t #p ✱ [⌜t = Node l x r⌝].
-Proof. iSteps. Qed.
+Proof. unfold is_tree, array. simpl. iSteps. Qed.
 
 Definition is_root_tree (t : root_tree) (v : val) : iProp Σ :=
   match t with
@@ -29,9 +31,9 @@ Definition is_root_tree (t : root_tree) (v : val) : iProp Σ :=
 
 #[export]
 Instance is_root_tree_root_hint (p : loc) (x : Z) (l_r l_l : val) t :
-HINT p ↦∗ [ #1; l_l; #x; l_r] ✱ [ l r ; is_tree l l_l ∗ is_tree r l_r ∗ ⌜t = Root l x r⌝]
+HINT ε₁ ✱ [ l r; (p +ₗ 0) ↦ #1 ∗ (p +ₗ 1) ↦ l_l ∗ (p +ₗ 2) ↦ #x ∗ (p +ₗ 3) ↦ l_r ∗ is_tree l l_l ∗ is_tree r l_r ∗ ⌜t = Root l x r⌝]
   ⊫ [id]; is_root_tree t #p ✱ [⌜t = Root l x r⌝].
-Proof. iSteps. Qed.
+Proof. unfold is_root_tree, array. simpl. iSteps. Qed.
 
 Fixpoint is_zipper (z : zipper) (v : val) : iProp Σ :=
   match z with
@@ -46,16 +48,14 @@ HINT ε₁ ✱ [- ; ⌜t = Done⌝] ⊫ [id]; is_zipper t NULL ✱ [⌜t = Done�
 Proof. iSteps. Qed.
 
 #[export]
-Instance is_zipper_nodel_hint (p : loc) (x : Z) (l_l l_r : val) t :
-HINT p ↦∗ [ #1; l_l; #x; l_r] ✱ [l r ; is_zipper l l_l ∗ is_tree r l_r ∗ ⌜t = NodeL l x r⌝]
-  ⊫ [id]; is_zipper t #p ✱ [⌜t = NodeL l x r⌝].
-Proof. iSteps. Qed.
-
-#[export]
-Instance is_zipper_noder_hint (p : loc) (x : Z) (l_l l_r : val) t :
-HINT p ↦∗ [ #2; l_l; #x; l_r] ✱ [l r ; is_tree l l_l ∗ is_zipper r l_r ∗ ⌜t = NodeR l x r⌝]
-  ⊫ [id]; is_zipper t #p ✱ [⌜t = NodeR l x r⌝].
-Proof. iSteps. Qed.
+Instance is_zipper_node_hint (p : loc) t :
+HINT ε₁ ✱ [ (tag : Z) z (x : Z) t' l_l l_r; (p +ₗ 0) ↦ #tag ∗ (p +ₗ 1) ↦ l_l ∗ (p +ₗ 2) ↦ #x ∗ (p +ₗ 3) ↦ l_r ∗
+  (if Z.eqb tag 1 then is_zipper z l_l ∗ is_tree t' l_r ∗ ⌜t = NodeL z x t'⌝
+                  else is_tree t' l_l ∗ is_zipper z l_r ∗ ⌜t = NodeR t' x z⌝ ∗ ⌜tag = 2⌝)]
+  ⊫ [id]; is_zipper t #p ✱ [(if Z.eqb tag 1 then ⌜t = NodeL z x t'⌝
+                                            else ⌜t = NodeR t' x z⌝)].
+Proof. iSteps as (? ? ? ? ? ?) "H1 H2 H3 H4 H5". destruct (x =? 1)%Z eqn:H6;
+       iDecompose "H5"; unfold array; iSteps. Qed.
 
 Notation "e1 '->tag'" :=
   (Load (BinOp OffsetOp e1%E (Val (LitV (LitInt (Z.of_nat 0))))))
